eqelim/consts.lean
@@ -1,0 +1,41 @@
+import ..term
+
+--@[reducible] def consts := (list term) × (list term)
+--
+--namespace consts
+--
+--meta instance has_to_format : has_to_format consts := by apply_instance
+
+--def weaker : consts → consts → Prop 
+--| ⟨eqs1,les1⟩ ⟨eqs2,les2⟩ := eqs1 ⊆ eqs2 ∧ les1 ⊆ les2 
+
+
+#exit
+
+@[reducible] def sat (c : consts) : Prop :=
+  ∃ v : nat → int, holds v c
+
+lemma sat_of_weaker {c1 c2} : 
+  weaker c1 c2 → sat c2 → sat c1 :=
+begin
+  intros h1 h2, cases h2 with v h2,
+  refine ⟨v,holds_of_weaker h1 h2⟩,
+end
+
+def unsat (c : consts) : Prop := ¬ c.sat 
+
+def append (c1 c2 : consts) : consts :=
+(c1.fst ++ c1.fst, c1.snd ++ c2.snd)
+
+def holds_append {v c1 c2} : 
+holds v c1 → holds v c2 → holds v (append c1 c2) := 
+begin
+  intros h1 h2, 
+  cases c1 with eqs1 les1,
+  cases c2 with eqs2 les2,
+  cases h1, cases h2,
+  constructor; rw list.forall_mem_append; 
+  constructor; assumption,
+end
+
+end consts
