eqelim/proof.lean
@@ -1,0 +1,172 @@
+import .sat
+
+@[omega] def comb : list term → list nat → term 
+| [] []     := ⟨0,[]⟩ 
+| [] (_::_) := ⟨0,[]⟩ 
+| (_::_) [] := ⟨0,[]⟩ 
+| (t::ts) (n::ns) := term.add (t.mul ↑n) (comb ts ns)
+
+lemma comb_holds {v} :
+  ∀ {ts} ns, (∀ t ∈ ts, 0 ≤ term.val v t) → (0 ≤ (comb ts ns).val v) 
+| [] []     h := by simp_omega
+| [] (_::_) h := by simp_omega
+| (_::_) [] h := by simp_omega
+| (t::ts) (n::ns) h :=
+  begin
+    simp_omega, apply add_nonneg, 
+    { apply mul_nonneg,
+      apply int.coe_nat_nonneg,
+      apply h _ (or.inl rfl) },
+    { apply comb_holds, 
+      apply list.forall_mem_of_forall_mem_cons h }
+  end
+
+def unsat_comb (ts ns) : Prop :=
+let t := comb ts ns in 
+if t.const < 0 ∧ ∀ x ∈ t.coeffs, x = (0 : int)
+then true
+else false
+
+lemma unsat_of_unsat_comb {eqs les : list term} (ns : list nat) :
+  (unsat_comb les ns) → unsat eqs les :=
+begin
+  intros h1 h2, cases h2 with v h2, 
+  have h3 := comb_holds ns h2.right,
+  by_cases h4 : (comb les ns).const < 0 ∧ 
+             ∀ x ∈ (comb les ns).coeffs, x = (0 : int),
+  { cases h4 with hl hr, 
+    cases (comb les ns) with b as,
+    simp_omega at h3, 
+    rw [val_aux_eq_zero hr, add_zero, ← not_lt] at h3,
+    apply h3 hl },
+  { simp only [unsat_comb] at h1, 
+    rw if_neg h4 at h1, exact h1 }
+end
+
+
+  #exit
+begin
+  intros h1 h2, simp only [correct] at h1,
+  cases h3 : comb_core ts p with t; rw h3 at h1, 
+  { cases h1 }, 
+  { simp at h1, cases h2 with v h2, 
+    have h5 := holds_comb h2 p _ h3, 
+    cases t with b as, simp_omega at h5,
+    rw [val_aux_eq_zero h1.right, add_zero, ← not_lt] at h5, 
+    apply h5 (int.neg_of_negative h1.left) }
+end
+
+
+
+#exit
+def correct (ts is) : Prop :=
+@option.rec_on _ (λ _, Prop) (comb_core ts p) false 
+(λ t, if t.const.negative ∧ (∀ x ∈ t.coeffs, x = (0 : int))
+      then true
+      else false)
+
+      #exit
+@[derive has_reflect]
+inductive proof : Type 
+| hyp   : nat → proof 
+| mul   : nat → proof → proof 
+| elim  : proof → proof → proof 
+
+-- | (proof.hyp m) :=
+-- | (proof.mul m p) :=
+-- | (proof.elim m p1 p2) := 
+
+def olc_rec : option term → (term → option term) → option term 
+| none      f := none 
+| (some lc) f := f lc
+
+lemma olc_rec_some (lc : term) (f) :
+  olc_rec (some lc) f = f lc := by refl 
+
+def comb_core (lcs : list term) : proof → option term 
+| (proof.hyp k)   := lcs.nth k
+| (proof.mul k p) := 
+  do lc ← comb_core p | none, some (lc.mul ↑k)
+| (proof.elim p1 p2) := 
+   do t1 ← comb_core p1, 
+      t2 ← comb_core p2, 
+      (some (term.add t1 t2))
+
+def int.negative : int → Prop 
+| (int.of_nat _) := false
+| -[1+ _]        := true
+
+lemma int.neg_of_negative {i : int} :
+  i.negative → i < 0 :=
+begin
+  cases i with m m; intro h1, cases h1,
+  cases m with m; tactic.exact_dec_trivial
+end
+
+instance int.decidable_negative : ∀ i : int, decidable i.negative 
+| (int.of_nat _) := decidable.false
+| -[1+ _]        := decidable.true
+
+
+lemma holds_comb {v lcs} (h0 : polytope.holds v lcs) : 
+  ∀ p t, comb_core lcs p = some t → 0 ≤ t.val v 
+| (proof.hyp m) t h1 := h0 _ (list.nth_mem h1)
+| (proof.mul m p) t h1 :=
+  begin
+    simp only [comb_core] at h1,
+    cases h3 : (comb_core lcs p) with s; rw h3 at h1,
+    { cases h1 },
+    { have h4 := holds_comb p s h3,
+      simp at h1, subst h1, simp only [term.val_mul],
+      apply int.mul_nonneg (int.coe_nat_nonneg _) h4 }
+  end
+| (proof.elim p1 p2) t h1 :=
+  begin
+    simp only [comb_core] at h1,
+    cases h3 : (comb_core lcs p1) with s; rw h3 at h1, cases h1,
+    cases h4 : (comb_core lcs p2) with u; rw h4 at h1, cases h1,
+    cases h1, rw term.val_add,
+    apply add_nonneg (holds_comb p1 s h3) (holds_comb p2 u h4), 
+  end
+
+lemma unsat_nil {t : term} :
+  false → 
+  polytope.unsat ([] : polytope) := λ h1, by cases h1
+
+lemma unsat_zero_le_neg {t : term} :
+  t.const < 0 → (∀ x : int, x ∈ t.coeffs → x = 0) → 
+  polytope.unsat ([t] : polytope) :=
+begin
+  intros h1 h2 h3, cases h3 with v h3,
+  have h4 := h3 _ (or.inl rfl),
+  cases t with c cfs,
+  simp only [term.val] at h4,
+  rw (val_aux_eq_zero h2) at h4,
+  simp at h4,
+  rw ← not_le at h1, apply (h1 h4),
+end
+
+def comb (lcs : list term) (p : proof) : list term :=
+option.rec_on (comb_core lcs p) ([] : list term) (λ t, [t])
+
+lemma unsat_of_unsat_comb {ts : list term} (p : proof) :
+  polytope.unsat (comb ts p) → polytope.unsat ts := 
+begin
+  intros h1 h2, apply h1, cases h2 with v h2, refine ⟨v,_⟩, 
+  simp only [comb], cases h3 : comb_core ts p, 
+  apply list.forall_mem_nil, simp [polytope.holds],
+  apply holds_comb h2 _ _ h3,
+end
+
+lemma unsat_of_correct {ts : list term} (p : proof) :
+  correct ts p → polytope.unsat ts :=
+begin
+  intros h1 h2, simp only [correct] at h1,
+  cases h3 : comb_core ts p with t; rw h3 at h1, 
+  { cases h1 }, 
+  { simp at h1, cases h2 with v h2, 
+    have h5 := holds_comb h2 p _ h3, 
+    cases t with b as, simp_omega at h5,
+    rw [val_aux_eq_zero h1.right, add_zero, ← not_lt] at h5, 
+    apply h5 (int.neg_of_negative h1.left) }
+end
