eqelim/search.lean
@@ -1,14 +1,14 @@
-import .proof
+import ..term 
 
 open tactic
 
-meta def find_contra : list (proof × term) → tactic proof
+meta def find_contra : list (list nat × term) → tactic (list nat)
 | []            := failed
 | ((π,⟨c,_⟩)::l) := if c < 0 then return π else find_contra l
 
 meta def trisect (m : nat) :  
-  list (proof × term) → (list (proof × term) × 
-  list (proof × term) × list (proof × term)) 
+  list (list nat × term) → (list (list nat × term) × 
+  list (list nat × term) × list (list nat × term)) 
 | [] := ([],[],[])
 | ((p,t)::pts) := 
   let (neg,zero,pos) := trisect pts in 
@@ -19,28 +19,29 @@ meta def trisect (m : nat) :
        else (neg,zero,(p,t)::pos)
 
 meta def elim_var_aux (m : nat) : 
-  ((proof × term) × (proof × term)) → tactic (proof × term) 
+  ((list nat × term) × (list nat × term)) → tactic (list nat × term) 
 | ((p1,t1), (p2,t2)) := 
   let n := int.nat_abs (t1.coeffs.get m) in
   let o := int.nat_abs (t2.coeffs.get m) in
   let lcm := (nat.lcm n o) in
   let n' := lcm / n in
   let o' := lcm / o in
-  return (proof.elim (p1.mul n') (p2.mul o'), term.add (t1.mul n') (t2.mul o'))
+  return (list.add (n' *₁ p1) (o' *₁ p2), 
+          term.add (t1.mul n') (t2.mul o'))
 
-meta def elim_var (m) (neg pos : list (proof × term)) : 
-  tactic (list (proof × term)) :=
+meta def elim_var (m) (neg pos : list (list nat × term)) : 
+  tactic (list (list nat × term)) :=
 let pairs := list.product neg pos in 
 monad.mapm (elim_var_aux m) pairs
 
-meta def search_core : nat → list (proof × term) → tactic proof 
+meta def search_core : nat → list (list nat × term) → tactic (list nat) 
 | 0 pts     := find_contra pts
 | (m+1) pts :=
   let (neg,zero,pos) := trisect m pts in
   do new ← elim_var m neg pos,
      search_core m (new ++ zero)
 
-meta def search (ts : list term) : tactic proof :=
+meta def search (ts : list term) : tactic (list nat) :=
 search_core 
   (ts.map (λ t : term, t.coeffs.length)).max  
-  (ts.map_with_idx (λ m t, (proof.hyp m, t)))
+  (ts.map_with_idx (λ m t, ([]{m ↦ 1}, t)))
