eqelim/tests.lean
@@ -1,0 +1,74 @@
+import .main 
+
+open tactic
+
+lemma false_of_empty_consts :
+  ¬(true ∧ true) → false :=
+begin intro h1, apply h1, exact_dec_trivial end
+
+meta def intro_all : tactic unit :=
+intros >> pexpr.apply ``(classical.by_contradiction _) >> 
+intro_fresh >> skip
+
+run_cmd mk_simp_attr `connectives
+attribute [connectives] 
+  classical.not_not
+  classical.not_and_distrib
+  classical.imp_iff_not_or
+  classical.iff_iff
+  not_or_distrib
+
+lemma int.not_eq {i j : int} :
+  ¬i = j ↔ (i + 1 ≤ j ∨ j + 1 ≤ i) :=
+begin
+  rw [le_antisymm_iff, classical.not_and_distrib,
+    not_le, int.lt_iff_add_one_le,
+    not_le, int.lt_iff_add_one_le, or.comm],
+end
+
+run_cmd mk_simp_attr `sugar
+attribute [sugar] 
+  not_le not_lt 
+  int.not_eq
+  int.lt_iff_add_one_le
+  zero_add add_zero
+  zero_mul mul_zero
+  or_false false_or
+  and_true true_and
+  ne ge gt mul_add add_mul 
+  mul_comm sub_eq_neg_add
+
+--meta def desugar := `[try {simp only with sugar at *}]
+
+local attribute [inline] interaction_monad_orelse
+
+meta def omega_decomp : tactic unit 
+| s := ((split_and <|> split_or) !; omega_decomp | 
+  (trace_state >> omega_core)) s
+
+meta def omega : tactic unit :=
+do intro_all,
+   `[try {simp only with connectives at *}],
+   `[try {simp only with sugar at *}],
+   pexpr.apply ``(false_of_empty_consts _),
+   omega_decomp
+
+set_option profiler true
+
+example {x y z w v : int} : 100 = x → x = y → y = z → z = w → w = v → v = 100 := by omega
+
+example : ∀ x : int, (x = 5 ∨ x = 7) → 2 < x := by omega
+example : ∀ x : int, x ≤ -x → x ≤ 0 := by omega
+example : ∀ x y : int, (x ≤ 5 ∧ y ≤ 3) → x + y ≤ 8 := by omega 
+example (x y z : int) : x < y → y < z → x < z := by omega 
+example (x y z : int) : x - y ≤ x - z → z ≤ y := by omega
+example : ∀ x : int, (x = -5 ∨ x = 7) → ¬x = 0 := by omega 
+example : ∀ x : int, 31 * x > 0 → x > 0 := by omega 
+example : ∀ x y : int, (-x - y < x - y) → (x - y < x + y) → (x > 0 ∧ y > 0) := by omega 
+example (x : int) : (x ≥ -1 ∧ x ≤ 1) → (x = -1 ∨ x = 0 ∨ x = 1):= by omega 
+example (x : int) : 5 * x = 5 → x = 1 := by omega 
+example : ∀ x y z : int, x = y → y = z → x = z := by omega 
+example : ∀ x : int, x < 349 ∨ x > 123 := by omega 
+example : ∀ x y : int, x ≤ 3 * y → 3 * x ≤ 9 * y := by omega 
+example : ∀ x : int, (x < 43 ∧ x > 513) → ¬x = x := by omega 
+example (x y z w : int) : x ≤ y → y ≤ z → z ≤ w → x ≤ w := by omega
