tactic.lean
@@ -1,9 +1,67 @@
 open tactic
 
+variables {α β : Type}
+
 meta def intro_fresh : tactic expr := 
 do n ← get_unused_name, intro n
 
 meta def pexpr.apply (x : pexpr) : tactic (list (name × expr)) :=
 to_expr x >>= apply
+
+meta def trace_target : tactic unit :=
+target >>= trace
+
+open expr
+
+meta def split_or_core : list expr → tactic unit 
+| [] := failed 
+| (x::xs) := 
+  do t ← infer_type x,
+     match t with 
+     | `(%%px ∨ %%qx) := 
+       (cases x >> skip) 
+       --trace "disj found" >> cases_core x >> trace "disj removed" >> skip
+       -- seq (pexpr.apply ``(or.elim %%x _ _) >> skip) (intro_fresh >> skip)
+     | _              := split_or_core xs
+     end
+
+meta def split_or : tactic unit := 
+local_context >>= split_or_core
+
+meta def split_and_core : list expr → tactic unit 
+| [] := failed 
+| (x::xs) := 
+  do t ← infer_type x,
+     match t with 
+     | `(%%px ∧ %%qx) := 
+       do np ← get_unused_name, 
+          nq ← get_unused_name, 
+          assertv np px (app (app (app `(@and.elim_left).to_expr px) qx) x),
+          assertv nq qx (app (app (app `(@and.elim_right).to_expr px) qx) x),
+          clear x
+     | _ := split_and_core xs
+     end
+
+meta def split_and : tactic unit := 
+local_context >>= split_and_core
+
+local attribute [inline] interaction_monad_orelse
+
+meta def commit (t1 t2 t3 : tactic unit) :=
+monad.cond ((t1 >> return tt) <|> return ff) t2 t3
+notation t1 `!>>` t2 `|` t3 := commit t1 t2 t3
+
+-- meta def try_solve (t1 t2 : tactic unit) : tactic unit := 
+-- t1 !>> (do n ← num_goals, if n = 0 then skip else t2), t2 
+-- infixr `?>>` : 500 := try_solve 
+
+meta def commit_seq (t1 t2 t3 : tactic unit) : tactic unit :=
+ do g::gs ← get_goals,
+    set_goals [g],
+    (t1 !>> (all_goals t2) | t3),
+    gs' ← get_goals,
+    set_goals (gs' ++ gs)
+
+notation t1 `!;` t2 `|` t3 : 500 := commit_seq t1 t2 t3
 
 
